timing/examples/x86_wcet_comparison/while_true_break/while_true_break_lifted.v
@@ -9,153 +9,149 @@ Require Import NArith.
 Require Import Lia.
 Open Scope N.
 
-Definition while_true_break_while_true_break_amd64 : program := fun _ a => match a with
+Definition while_true_break_amd64 : program := fun _ a => match a with
 
-(* 0x00101140: MOV EDX,EDI *)
-(*    1052992: MOV EDX,EDI *)
-| 0x101140 => Some (2,
-	Move R_RDX (Cast CAST_UNSIGNED 64 (Extract 31 0 (Var R_RDI))) $;
-	Move R_RDX (Cast CAST_UNSIGNED 64 (Extract 31 0 (Var R_RDX)))
+(* 0x001011a0: MOV RDX,RDI *)
+(*          0: MOV RDX,RDI *)
+| 0x0 => Some (3,
+	Move R_RDX (Var R_RDI)
 )
 
-(* 0x00101142: LEA ECX,[RDI + RDI*0x1] *)
-(*    1052994: LEA ECX,[RDI + RDI*0x1] *)
-| 0x101142 => Some (3,
-	Move (V_TEMP 0x4600) (BinOp OP_TIMES (Var R_RDI) (Word 0x1 64)) $;
-	Move (V_TEMP 0x4700) (BinOp OP_PLUS (Var R_RDI) (Var (V_TEMP 0x4600))) $;
-	Move R_RCX (Cast CAST_LOW 64 (BinOp OP_RSHIFT (Var (V_TEMP 0x4700)) (Word 0 64))) $;
-	Move R_RCX (Cast CAST_UNSIGNED 64 (Extract 31 0 (Var R_RCX)))
+(* 0x001011a3: LEA RCX,[RDI + RDI*0x1] *)
+(*          3: LEA RCX,[RDI + RDI*0x1] *)
+| 0x3 => Some (4,
+	Move (V_TEMP 0x4980) (BinOp OP_TIMES (Var R_RDI) (Word 0x1 64)) $;
+	Move (V_TEMP 0x4a80) (BinOp OP_PLUS (Var R_RDI) (Var (V_TEMP 0x4980))) $;
+	Move R_RCX (Var (V_TEMP 0x4a80))
 )
 
-(* 0x00101145: MOV EAX,EDI *)
-(*    1052997: MOV EAX,EDI *)
-| 0x101145 => Some (2,
-	Move R_RAX (Cast CAST_UNSIGNED 64 (Extract 31 0 (Var R_RDI))) $;
-	Move R_RAX (Cast CAST_UNSIGNED 64 (Extract 31 0 (Var R_RAX)))
+(* 0x001011a7: MOV RAX,RDI *)
+(*          7: MOV RAX,RDI *)
+| 0x7 => Some (3,
+	Move R_RAX (Var R_RDI)
 )
 
-(* 0x00101147: IMUL EDX,EDI *)
-(*    1052999: IMUL EDX,EDI *)
-| 0x101147 => Some (3,
-	Move (V_TEMP 0x33e80) (Cast CAST_SIGNED 64 (Extract 31 0 (Var R_RDX))) $;
-	Move (V_TEMP 0x33f00) (Cast CAST_SIGNED 64 (Extract 31 0 (Var R_RDI))) $;
-	Move (V_TEMP 0x34000) (BinOp OP_TIMES (Var (V_TEMP 0x33e80)) (Var (V_TEMP 0x33f00))) $;
-	Move R_RDX (Cast CAST_LOW 64 (BinOp OP_RSHIFT (Var (V_TEMP 0x34000)) (Word 0 64))) $;
-	Move (V_TEMP 0x34180) (Cast CAST_LOW 32 (BinOp OP_RSHIFT (Var (V_TEMP 0x34000)) (Word 32 64))) $;
-	Move (V_TEMP 0x16080) (Cast CAST_SIGNED 64 (Extract 31 0 (Var R_RDX))) $;
-	Move R_CF (Cast CAST_LOW 1 (BinOp OP_NEQ (Var (V_TEMP 0x16080)) (Var (V_TEMP 0x34000)))) $;
-	Move R_OF (Cast CAST_LOW 1 (Var R_CF)) $;
-	Move R_RDX (Cast CAST_UNSIGNED 64 (Extract 31 0 (Var R_RDX)))
+(* 0x001011aa: IMUL RDX,RDI *)
+(*         10: IMUL RDX,RDI *)
+| 0xa => Some (4,
+	Move (V_TEMP 0x4b500) (Cast CAST_SIGNED 128 (Var R_RDX)) $;
+	Move (V_TEMP 0x4b580) (Cast CAST_SIGNED 128 (Var R_RDI)) $;
+	Move (V_TEMP 0x4b680) (BinOp OP_TIMES (Var (V_TEMP 0x4b500)) (Var (V_TEMP 0x4b580))) $;
+	Move R_RDX (BinOp OP_TIMES (Var R_RDX) (Var R_RDI)) $;
+	Move (V_TEMP 0x4b800) (Cast CAST_LOW 64 (BinOp OP_RSHIFT (Var (V_TEMP 0x4b680)) (Word 64 128))) $;
+	Move (V_TEMP 0x2d200) (Cast CAST_SIGNED 128 (Var R_RDX)) $;
+	Move R_CF (Cast CAST_LOW 1 (BinOp OP_NEQ (Var (V_TEMP 0x2d200)) (Var (V_TEMP 0x4b680)))) $;
+	Move R_OF (Cast CAST_LOW 1 (Var R_CF))
 )
 
-(* 0x0010114a: CMP ECX,EDX *)
-(*    1053002: CMP ECX,EDX *)
-| 0x10114a => Some (2,
-	Move (V_TEMP 0x27e00) (Extract 31 0 (Var R_RCX)) $;
-	Move R_CF (Cast CAST_LOW 1 (BinOp OP_LT (Var (V_TEMP 0x27e00)) (Extract 31 0 (Var R_RDX)))) $;
-	Move R_OF (Cast CAST_LOW 1 (Cast CAST_LOW 8 (BinOp OP_AND (BinOp OP_XOR (BinOp OP_AND (BinOp OP_RSHIFT (Var (V_TEMP 0x27e00)) (Word 31 32)) (Word 1 32)) (BinOp OP_AND (BinOp OP_RSHIFT (BinOp OP_MINUS (Var (V_TEMP 0x27e00)) (Extract 31 0 (Var R_RDX))) (Word 31 32)) (Word 1 32))) (BinOp OP_XOR (BinOp OP_XOR (BinOp OP_AND (BinOp OP_RSHIFT (BinOp OP_MINUS (Var (V_TEMP 0x27e00)) (Extract 31 0 (Var R_RDX))) (Word 31 32)) (Word 1 32)) (BinOp OP_AND (BinOp OP_RSHIFT (Extract 31 0 (Var R_RDX)) (Word 31 32)) (Word 1 32))) (Word 1 32))))) $;
-	Move (V_TEMP 0x27f00) (BinOp OP_MINUS (Var (V_TEMP 0x27e00)) (Extract 31 0 (Var R_RDX))) $;
-	Move R_SF (Cast CAST_LOW 1 (BinOp OP_SLT (Var (V_TEMP 0x27f00)) (Word 0x0 32))) $;
-	Move R_ZF (Cast CAST_LOW 1 (BinOp OP_EQ (Var (V_TEMP 0x27f00)) (Word 0x0 32))) $;
-	Move (V_TEMP 0x15100) (BinOp OP_AND (Var (V_TEMP 0x27f00)) (Word 0xff 32)) $;
-	Move (V_TEMP 0x15180) (Cast CAST_LOW 8 (UnOp OP_POPCOUNT (Var (V_TEMP 0x15100)))) $;
-	Move (V_TEMP 0x15200) (BinOp OP_AND (Var (V_TEMP 0x15180)) (Word 0x1 8)) $;
-	Move R_PF (Cast CAST_LOW 1 (BinOp OP_EQ (Var (V_TEMP 0x15200)) (Word 0x0 8)))
+(* 0x001011ae: CMP RCX,RDX *)
+(*         14: CMP RCX,RDX *)
+| 0xe => Some (3,
+	Move (V_TEMP 0x3f100) (Var R_RCX) $;
+	Move R_CF (Cast CAST_LOW 1 (BinOp OP_LT (Var (V_TEMP 0x3f100)) (Var R_RDX))) $;
+	Move R_OF (Cast CAST_LOW 1 (Cast CAST_LOW 8 (BinOp OP_AND (BinOp OP_XOR (BinOp OP_AND (BinOp OP_RSHIFT (Var (V_TEMP 0x3f100)) (Word 63 64)) (Word 1 64)) (BinOp OP_AND (BinOp OP_RSHIFT (BinOp OP_MINUS (Var (V_TEMP 0x3f100)) (Var R_RDX)) (Word 63 64)) (Word 1 64))) (BinOp OP_XOR (BinOp OP_XOR (BinOp OP_AND (BinOp OP_RSHIFT (BinOp OP_MINUS (Var (V_TEMP 0x3f100)) (Var R_RDX)) (Word 63 64)) (Word 1 64)) (BinOp OP_AND (BinOp OP_RSHIFT (Var R_RDX) (Word 63 64)) (Word 1 64))) (Word 1 64))))) $;
+	Move (V_TEMP 0x3f200) (BinOp OP_MINUS (Var (V_TEMP 0x3f100)) (Var R_RDX)) $;
+	Move R_SF (Cast CAST_LOW 1 (BinOp OP_SLT (Var (V_TEMP 0x3f200)) (Word 0x0 64))) $;
+	Move R_ZF (Cast CAST_LOW 1 (BinOp OP_EQ (Var (V_TEMP 0x3f200)) (Word 0x0 64))) $;
+	Move (V_TEMP 0x2c280) (BinOp OP_AND (Var (V_TEMP 0x3f200)) (Word 0xff 64)) $;
+	Move (V_TEMP 0x2c300) (Cast CAST_LOW 8 (UnOp OP_POPCOUNT (Var (V_TEMP 0x2c280)))) $;
+	Move (V_TEMP 0x2c380) (BinOp OP_AND (Var (V_TEMP 0x2c300)) (Word 0x1 8)) $;
+	Move R_PF (Cast CAST_LOW 1 (BinOp OP_EQ (Var (V_TEMP 0x2c380)) (Word 0x0 8)))
 )
 
-(* 0x0010114c: JGE 0x0010115f *)
-(*    1053004: JGE 0x0010115f *)
-| 0x10114c => Some (2,
-	Move (V_TEMP 0xeb80) (BinOp OP_EQ (Var R_OF) (Var R_SF)) $;
-	If (Cast CAST_LOW 1 (Var (V_TEMP 0xeb80))) (
-		Jmp (Word 0x10115f 64)
+(* 0x001011b1: JNC 0x001011d4 *)
+(*         17: JNC 0x001011d4 *)
+| 0x11 => Some (2,
+	Move (V_TEMP 0x12780) (UnOp OP_NOT (Var R_CF)) $;
+	If (Cast CAST_LOW 1 (Var (V_TEMP 0x12780))) (
+		Jmp (Word 0x34 64)
 	) (* else *) (
 		Nop
 	)
 )
 
-(* 0x0010114e: NOP *)
-(*    1053006: NOP *)
-| 0x10114e => Some (2,
+(* 0x001011b3: NOP dword ptr CS:[RAX + RAX*0x1] *)
+(*         19: NOP dword ptr CS:[RAX + RAX*0x1] *)
+| 0x13 => Some (11,
+	Move (V_TEMP 0x5580) (BinOp OP_TIMES (Var R_RAX) (Word 0x1 64)) $;
+	Move (V_TEMP 0x5680) (BinOp OP_PLUS (Var R_RAX) (Var (V_TEMP 0x5580)))
+)
+
+(* 0x001011be: NOP *)
+(*         30: NOP *)
+| 0x1e => Some (2,
 	Nop
 )
 
-(* 0x00101150: SUB EAX,0x1 *)
-(*    1053008: SUB EAX,0x1 *)
-| 0x101150 => Some (3,
-	Move R_CF (Cast CAST_LOW 1 (BinOp OP_LT (Extract 31 0 (Var R_RAX)) (Word 0x1 32))) $;
-	Move R_OF (Cast CAST_LOW 1 (Cast CAST_LOW 8 (BinOp OP_AND (BinOp OP_XOR (BinOp OP_AND (BinOp OP_RSHIFT (Extract 31 0 (Var R_RAX)) (Word 31 32)) (Word 1 32)) (BinOp OP_AND (BinOp OP_RSHIFT (BinOp OP_MINUS (Extract 31 0 (Var R_RAX)) (Word 0x1 32)) (Word 31 32)) (Word 1 32))) (BinOp OP_XOR (BinOp OP_XOR (BinOp OP_AND (BinOp OP_RSHIFT (BinOp OP_MINUS (Extract 31 0 (Var R_RAX)) (Word 0x1 32)) (Word 31 32)) (Word 1 32)) (BinOp OP_AND (BinOp OP_RSHIFT (Word 0x1 32) (Word 31 32)) (Word 1 32))) (Word 1 32))))) $;
-	Move R_RAX (Cast CAST_SIGNED 64 (BinOp OP_MINUS (Extract 31 0 (Var R_RAX)) (Word 0x1 32))) $;
-	Move R_RAX (Cast CAST_UNSIGNED 64 (Extract 31 0 (Var R_RAX))) $;
-	Move R_SF (Cast CAST_LOW 1 (BinOp OP_SLT (Extract 31 0 (Var R_RAX)) (Word 0x0 32))) $;
-	Move R_ZF (Cast CAST_LOW 1 (BinOp OP_EQ (Extract 31 0 (Var R_RAX)) (Word 0x0 32))) $;
-	Move (V_TEMP 0x15100) (BinOp OP_AND (Extract 31 0 (Var R_RAX)) (Word 0xff 32)) $;
-	Move (V_TEMP 0x15180) (Cast CAST_LOW 8 (UnOp OP_POPCOUNT (Var (V_TEMP 0x15100)))) $;
-	Move (V_TEMP 0x15200) (BinOp OP_AND (Var (V_TEMP 0x15180)) (Word 0x1 8)) $;
-	Move R_PF (Cast CAST_LOW 1 (BinOp OP_EQ (Var (V_TEMP 0x15200)) (Word 0x0 8)))
+(* 0x001011c0: SUB RAX,0x1 *)
+(*         32: SUB RAX,0x1 *)
+| 0x20 => Some (4,
+	Move R_CF (Cast CAST_LOW 1 (BinOp OP_LT (Var R_RAX) (Word 0x1 64))) $;
+	Move R_OF (Cast CAST_LOW 1 (Cast CAST_LOW 8 (BinOp OP_AND (BinOp OP_XOR (BinOp OP_AND (BinOp OP_RSHIFT (Var R_RAX) (Word 63 64)) (Word 1 64)) (BinOp OP_AND (BinOp OP_RSHIFT (BinOp OP_MINUS (Var R_RAX) (Word 0x1 64)) (Word 63 64)) (Word 1 64))) (BinOp OP_XOR (BinOp OP_XOR (BinOp OP_AND (BinOp OP_RSHIFT (BinOp OP_MINUS (Var R_RAX) (Word 0x1 64)) (Word 63 64)) (Word 1 64)) (BinOp OP_AND (BinOp OP_RSHIFT (Word 0x1 64) (Word 63 64)) (Word 1 64))) (Word 1 64))))) $;
+	Move R_RAX (BinOp OP_MINUS (Var R_RAX) (Word 0x1 64)) $;
+	Move R_SF (Cast CAST_LOW 1 (BinOp OP_SLT (Var R_RAX) (Word 0x0 64))) $;
+	Move R_ZF (Cast CAST_LOW 1 (BinOp OP_EQ (Var R_RAX) (Word 0x0 64))) $;
+	Move (V_TEMP 0x2c280) (BinOp OP_AND (Var R_RAX) (Word 0xff 64)) $;
+	Move (V_TEMP 0x2c300) (Cast CAST_LOW 8 (UnOp OP_POPCOUNT (Var (V_TEMP 0x2c280)))) $;
+	Move (V_TEMP 0x2c380) (BinOp OP_AND (Var (V_TEMP 0x2c300)) (Word 0x1 8)) $;
+	Move R_PF (Cast CAST_LOW 1 (BinOp OP_EQ (Var (V_TEMP 0x2c380)) (Word 0x0 8)))
 )
 
-(* 0x00101153: MOV ECX,EAX *)
-(*    1053011: MOV ECX,EAX *)
-| 0x101153 => Some (2,
-	Move R_RCX (Cast CAST_UNSIGNED 64 (Extract 31 0 (Var R_RAX))) $;
-	Move R_RCX (Cast CAST_UNSIGNED 64 (Extract 31 0 (Var R_RCX)))
+(* 0x001011c4: MOV RDX,RAX *)
+(*         36: MOV RDX,RAX *)
+| 0x24 => Some (3,
+	Move R_RDX (Var R_RAX)
 )
 
-(* 0x00101155: LEA EDX,[RAX + RAX*0x1] *)
-(*    1053013: LEA EDX,[RAX + RAX*0x1] *)
-| 0x101155 => Some (3,
-	Move (V_TEMP 0x4600) (BinOp OP_TIMES (Var R_RAX) (Word 0x1 64)) $;
-	Move (V_TEMP 0x4700) (BinOp OP_PLUS (Var R_RAX) (Var (V_TEMP 0x4600))) $;
-	Move R_RDX (Cast CAST_LOW 64 (BinOp OP_RSHIFT (Var (V_TEMP 0x4700)) (Word 0 64))) $;
-	Move R_RDX (Cast CAST_UNSIGNED 64 (Extract 31 0 (Var R_RDX)))
+(* 0x001011c7: LEA RCX,[RAX + RAX*0x1] *)
+(*         39: LEA RCX,[RAX + RAX*0x1] *)
+| 0x27 => Some (4,
+	Move (V_TEMP 0x4980) (BinOp OP_TIMES (Var R_RAX) (Word 0x1 64)) $;
+	Move (V_TEMP 0x4a80) (BinOp OP_PLUS (Var R_RAX) (Var (V_TEMP 0x4980))) $;
+	Move R_RCX (Var (V_TEMP 0x4a80))
 )
 
-(* 0x00101158: IMUL ECX,EAX *)
-(*    1053016: IMUL ECX,EAX *)
-| 0x101158 => Some (3,
-	Move (V_TEMP 0x33e80) (Cast CAST_SIGNED 64 (Extract 31 0 (Var R_RCX))) $;
-	Move (V_TEMP 0x33f00) (Cast CAST_SIGNED 64 (Extract 31 0 (Var R_RAX))) $;
-	Move (V_TEMP 0x34000) (BinOp OP_TIMES (Var (V_TEMP 0x33e80)) (Var (V_TEMP 0x33f00))) $;
-	Move R_RCX (Cast CAST_LOW 64 (BinOp OP_RSHIFT (Var (V_TEMP 0x34000)) (Word 0 64))) $;
-	Move (V_TEMP 0x34180) (Cast CAST_LOW 32 (BinOp OP_RSHIFT (Var (V_TEMP 0x34000)) (Word 32 64))) $;
-	Move (V_TEMP 0x16080) (Cast CAST_SIGNED 64 (Extract 31 0 (Var R_RCX))) $;
-	Move R_CF (Cast CAST_LOW 1 (BinOp OP_NEQ (Var (V_TEMP 0x16080)) (Var (V_TEMP 0x34000)))) $;
-	Move R_OF (Cast CAST_LOW 1 (Var R_CF)) $;
-	Move R_RCX (Cast CAST_UNSIGNED 64 (Extract 31 0 (Var R_RCX)))
+(* 0x001011cb: IMUL RDX,RAX *)
+(*         43: IMUL RDX,RAX *)
+| 0x2b => Some (4,
+	Move (V_TEMP 0x4b500) (Cast CAST_SIGNED 128 (Var R_RDX)) $;
+	Move (V_TEMP 0x4b580) (Cast CAST_SIGNED 128 (Var R_RAX)) $;
+	Move (V_TEMP 0x4b680) (BinOp OP_TIMES (Var (V_TEMP 0x4b500)) (Var (V_TEMP 0x4b580))) $;
+	Move R_RDX (BinOp OP_TIMES (Var R_RDX) (Var R_RAX)) $;
+	Move (V_TEMP 0x4b800) (Cast CAST_LOW 64 (BinOp OP_RSHIFT (Var (V_TEMP 0x4b680)) (Word 64 128))) $;
+	Move (V_TEMP 0x2d200) (Cast CAST_SIGNED 128 (Var R_RDX)) $;
+	Move R_CF (Cast CAST_LOW 1 (BinOp OP_NEQ (Var (V_TEMP 0x2d200)) (Var (V_TEMP 0x4b680)))) $;
+	Move R_OF (Cast CAST_LOW 1 (Var R_CF))
 )
 
-(* 0x0010115b: CMP ECX,EDX *)
-(*    1053019: CMP ECX,EDX *)
-| 0x10115b => Some (2,
-	Move (V_TEMP 0x27e00) (Extract 31 0 (Var R_RCX)) $;
-	Move R_CF (Cast CAST_LOW 1 (BinOp OP_LT (Var (V_TEMP 0x27e00)) (Extract 31 0 (Var R_RDX)))) $;
-	Move R_OF (Cast CAST_LOW 1 (Cast CAST_LOW 8 (BinOp OP_AND (BinOp OP_XOR (BinOp OP_AND (BinOp OP_RSHIFT (Var (V_TEMP 0x27e00)) (Word 31 32)) (Word 1 32)) (BinOp OP_AND (BinOp OP_RSHIFT (BinOp OP_MINUS (Var (V_TEMP 0x27e00)) (Extract 31 0 (Var R_RDX))) (Word 31 32)) (Word 1 32))) (BinOp OP_XOR (BinOp OP_XOR (BinOp OP_AND (BinOp OP_RSHIFT (BinOp OP_MINUS (Var (V_TEMP 0x27e00)) (Extract 31 0 (Var R_RDX))) (Word 31 32)) (Word 1 32)) (BinOp OP_AND (BinOp OP_RSHIFT (Extract 31 0 (Var R_RDX)) (Word 31 32)) (Word 1 32))) (Word 1 32))))) $;
-	Move (V_TEMP 0x27f00) (BinOp OP_MINUS (Var (V_TEMP 0x27e00)) (Extract 31 0 (Var R_RDX))) $;
-	Move R_SF (Cast CAST_LOW 1 (BinOp OP_SLT (Var (V_TEMP 0x27f00)) (Word 0x0 32))) $;
-	Move R_ZF (Cast CAST_LOW 1 (BinOp OP_EQ (Var (V_TEMP 0x27f00)) (Word 0x0 32))) $;
-	Move (V_TEMP 0x15100) (BinOp OP_AND (Var (V_TEMP 0x27f00)) (Word 0xff 32)) $;
-	Move (V_TEMP 0x15180) (Cast CAST_LOW 8 (UnOp OP_POPCOUNT (Var (V_TEMP 0x15100)))) $;
-	Move (V_TEMP 0x15200) (BinOp OP_AND (Var (V_TEMP 0x15180)) (Word 0x1 8)) $;
-	Move R_PF (Cast CAST_LOW 1 (BinOp OP_EQ (Var (V_TEMP 0x15200)) (Word 0x0 8)))
+(* 0x001011cf: CMP RCX,RDX *)
+(*         47: CMP RCX,RDX *)
+| 0x2f => Some (3,
+	Move (V_TEMP 0x3f100) (Var R_RCX) $;
+	Move R_CF (Cast CAST_LOW 1 (BinOp OP_LT (Var (V_TEMP 0x3f100)) (Var R_RDX))) $;
+	Move R_OF (Cast CAST_LOW 1 (Cast CAST_LOW 8 (BinOp OP_AND (BinOp OP_XOR (BinOp OP_AND (BinOp OP_RSHIFT (Var (V_TEMP 0x3f100)) (Word 63 64)) (Word 1 64)) (BinOp OP_AND (BinOp OP_RSHIFT (BinOp OP_MINUS (Var (V_TEMP 0x3f100)) (Var R_RDX)) (Word 63 64)) (Word 1 64))) (BinOp OP_XOR (BinOp OP_XOR (BinOp OP_AND (BinOp OP_RSHIFT (BinOp OP_MINUS (Var (V_TEMP 0x3f100)) (Var R_RDX)) (Word 63 64)) (Word 1 64)) (BinOp OP_AND (BinOp OP_RSHIFT (Var R_RDX) (Word 63 64)) (Word 1 64))) (Word 1 64))))) $;
+	Move (V_TEMP 0x3f200) (BinOp OP_MINUS (Var (V_TEMP 0x3f100)) (Var R_RDX)) $;
+	Move R_SF (Cast CAST_LOW 1 (BinOp OP_SLT (Var (V_TEMP 0x3f200)) (Word 0x0 64))) $;
+	Move R_ZF (Cast CAST_LOW 1 (BinOp OP_EQ (Var (V_TEMP 0x3f200)) (Word 0x0 64))) $;
+	Move (V_TEMP 0x2c280) (BinOp OP_AND (Var (V_TEMP 0x3f200)) (Word 0xff 64)) $;
+	Move (V_TEMP 0x2c300) (Cast CAST_LOW 8 (UnOp OP_POPCOUNT (Var (V_TEMP 0x2c280)))) $;
+	Move (V_TEMP 0x2c380) (BinOp OP_AND (Var (V_TEMP 0x2c300)) (Word 0x1 8)) $;
+	Move R_PF (Cast CAST_LOW 1 (BinOp OP_EQ (Var (V_TEMP 0x2c380)) (Word 0x0 8)))
 )
 
-(* 0x0010115d: JG 0x00101150 *)
-(*    1053021: JG 0x00101150 *)
-| 0x10115d => Some (2,
-	Move (V_TEMP 0xed80) (UnOp OP_NOT (Var R_ZF)) $;
-	Move (V_TEMP 0xee00) (BinOp OP_EQ (Var R_OF) (Var R_SF)) $;
-	Move (V_TEMP 0xef00) (BinOp OP_AND (Var (V_TEMP 0xed80)) (Var (V_TEMP 0xee00))) $;
-	If (Cast CAST_LOW 1 (Var (V_TEMP 0xef00))) (
-		Jmp (Word 0x101150 64)
+(* 0x001011d2: JC 0x001011c0 *)
+(*         50: JC 0x001011c0 *)
+| 0x32 => Some (2,
+	If (Cast CAST_LOW 1 (Var R_CF)) (
+		Jmp (Word 0x20 64)
 	) (* else *) (
 		Nop
 	)
 )
 
-(* 0x0010115f: RET *)
-(*    1053023: RET *)
-| 0x10115f => Some (1,
+(* 0x001011d4: RET *)
+(*         52: RET *)
+| 0x34 => Some (1,
 	Move R_RIP (Load (Var V_MEM64) (Var R_RSP) LittleE 8) $;
 	Move R_RSP (BinOp OP_PLUS (Var R_RSP) (Word 0x8 64)) $;
 	Jmp (Var R_RIP)
@@ -170,6 +166,5 @@ end.
  *                                                         *
  * * * * * * * * * * * * * * * * * * * * * * * * * * * * * *)
 
-Theorem welltyped: welltyped_prog x64typctx while_true_break_while_true_break_amd64.
+Theorem welltyped: welltyped_prog x64typctx while_true_break_amd64.
 Proof. Picinae_typecheck. Qed.
-
