timing/examples/x86_wcet_comparison/while_true_break/while_true_break_proofs.v
@@ -1,0 +1,193 @@
+Require Import while_true_break_lifted.
+Require Import AMD64Timing.
+Import X64Notations.
+Require Import TimingAutomation.
+Require Import Arith.
+
+Module TimingProof (cpu : amd64CPUTimingBehavior).
+Import cpu.
+
+Module Program_while_true_break <: ProgramInformation.
+    Definition entry_addr : N := 0x0.
+
+    Definition exits (t:trace) : bool :=
+        match t with (Addr a,_)::_ => match a with
+        | 0x34 => true
+        | _ => false
+    end | _ => false end.
+
+    Definition time_of_addr (s : store) (a : addr) : N :=
+        match a with
+        (* 0x0 : MOV RDX,RDI *)
+        | 0x0 => mov_r64_r64
+        (* 0x3 : LEA RCX,[RDI + RDI*0x1] *)
+        | 0x3 => lea_r64_addr
+        (* 0x7 : MOV RAX,RDI *)
+        | 0x7 => mov_r64_r64
+        (* 0xa : IMUL RDX,RDI *)
+        | 0xa => imul_r64_r64
+        (* 0xe : CMP RCX,RDX *)
+        | 0xe => cmp_r64_r64
+        (* 0x11 : JNC 0x... *)
+        | 0x11 => jnc_addr
+        (* 0x13 : NOP dword ptr CS:[RAX + RAX*0x1] (lifted to address calc) *)
+        | 0x13 => nop
+        (* 0x1e : NOP *)
+        | 0x1e => nop
+        (* 0x20 : SUB RAX,0x1 *)
+        | 0x20 => sub_r64_i
+        (* 0x24 : MOV RDX,RAX *)
+        | 0x24 => mov_r64_r64
+        (* 0x27 : LEA RCX,[RAX + RAX*0x1] *)
+        | 0x27 => lea_r64_addr
+        (* 0x2b : IMUL RDX,RAX *)
+        | 0x2b => imul_r64_r64
+        (* 0x2f : CMP RCX,RDX *)
+        | 0x2f => cmp_r64_r64
+        (* 0x32 : JC 0x... *)
+        | 0x32 => jc_addr
+        (* 0x34 : RET *)
+        | 0x34 => ret
+        | _ => time_inf
+        end.
+
+    Definition lifted_prog := while_true_break_amd64.
+End Program_while_true_break.
+
+Module AMD64Timing := AMD64Timing cpu Program_while_true_break.
+Module while_true_breakAuto := AMD64TimingAutomation AMD64Timing.
+Import Program_while_true_break while_true_breakAuto.
+
+Definition time_of_while_true_break (n : N) (t : trace) :=
+  cycle_count_of_trace t <=
+    mov_r64_r64 + lea_r64_addr + mov_r64_r64 + imul_r64_r64 + cmp_r64_r64 +
+    jnc_addr +
+    if (n * n <=? n + n) then ret else (
+        nop + nop +
+        (* loop iters *)
+        (n - 2) * (
+            sub_r64_i + mov_r64_r64 + lea_r64_addr + imul_r64_r64 +
+            cmp_r64_r64 + jc_addr
+        ) + ret
+    ).
+
+Definition while_true_break_timing_invs (n : N) (t:trace) : option Prop :=
+match t with (Addr a, s) :: t' => match a with
+| 0x0 => Some (
+    s R_RDI = n /\ 0 <= n < 1000 /\
+    cycle_count_of_trace t' = 0
+  )
+| 0x20 => Some (
+    3 <= n < 1000 /\
+    3 <= s R_RAX <= n /\
+    n * n <=? n + n = false /\
+    cycle_count_of_trace t' <=
+        mov_r64_r64 + lea_r64_addr + mov_r64_r64 + imul_r64_r64 + cmp_r64_r64 +
+        jnc_addr + nop + nop +
+        (* loop iters *)
+        (n - s R_RAX) * (
+            sub_r64_i + mov_r64_r64 + lea_r64_addr + imul_r64_r64 +
+            cmp_r64_r64 + jc_addr
+        )
+  )
+| 0x34 => Some (time_of_while_true_break n t)
+| _ => None end | _ => None end.
+
+Lemma Contra : forall n,
+    n * n <= n + n -> n <= 2.
+Proof.
+    induction n using N.peano_ind; intros.
+        lia.
+    lia.
+Qed.
+
+Theorem while_true_break_timing:
+  forall s t s' x' n
+         (* boilerplate *)
+         (ENTRY: startof t (x',s') = (Addr entry_addr, s))
+         (MDL: models x64typctx s)
+         (* bindings *)
+         (RDI: s R_RDI = n)
+         (EDI: 0 <= n < 1000),
+  satisfies_all
+    lifted_prog
+    (while_true_break_timing_invs n)
+    exits
+  ((x',s')::t).
+Proof using.
+    intros.
+    apply prove_invs.
+
+    Local Ltac step := tstep x64_step.
+    simpl. rewrite ENTRY. unfold entry_addr. step.
+    repeat split; auto; lia.
+
+    intros.
+    eapply startof_prefix in ENTRY; try eassumption.
+    eapply preservation_exec_prog in MDL;
+        try eassumption; [idtac|apply welltyped].
+    clear - ENTRY PRE MDL. rename t1 into t. rename s1 into s'.
+
+    destruct_inv 64 PRE.
+
+    - destruct PRE as (RDI & Bounds & Cycles).
+        repeat step.
+        rewrite N.mod_small in BC by lia.
+        assert (n * n < 2^64). {
+            change (2^64) with (2^32 * 2^32).
+            rewrite <- N.square_lt_mono. lia.
+        }
+        rewrite N.mod_small in BC by lia.
+        split.
+            destruct n using N.peano_ind. discriminate.
+            destruct n using N.peano_ind. discriminate.
+            destruct n using N.peano_ind. discriminate.
+            lia.
+        split.
+            destruct n using N.peano_ind. discriminate.
+            destruct n using N.peano_ind. discriminate.
+            lia.
+        split. lia.
+        hammer.
+        rewrite N.mod_small in BC by lia.
+        assert (n * n < 2^64). {
+            change (2^64) with (2^32 * 2^32).
+            rewrite <- N.square_lt_mono. lia.
+        }
+        rewrite N.mod_small in BC by lia.
+        replace (n * n <=? n + n) with true by lia.
+        hammer.
+    - destruct PRE as (NBounds & Bounds & Path & Cycles).
+        repeat step.
+        split. assumption.
+        split.
+            rewrite msub_nowrap by (psimpl; lia). psimpl. split; [| lia].
+            destruct (s' R_RAX) using N.peano_ind. lia.
+            destruct n0 using N.peano_ind. lia.
+            destruct n0 using N.peano_ind. clear IHn0 IHn1.
+                cbv [N.succ Pos.succ] in BC. psimpl in BC. discriminate.
+            destruct n0 using N.peano_ind. clear IHn0 IHn1 IHn2.
+                cbv [N.succ Pos.succ] in BC. psimpl in BC. discriminate.
+                clear. lia.
+        split. assumption.
+        hammer.
+            rewrite msub_nowrap by (psimpl; lia).
+            psimpl. rewrite N.sub_sub_distr by lia. lia.
+
+        rewrite Path.
+        hammer.
+        rewrite msub_nowrap, msub_nowrap in BC by lia.
+        psimpl in BC. rewrite N.mod_small in BC by lia.
+        rewrite N.mod_small in BC.
+        replace (s' R_RAX - 2 + s' R_RAX) with
+            ((s' R_RAX - 1) + (s' R_RAX - 1)) in BC by lia.
+        apply N.ltb_ge, Contra in BC.
+        assert (s' R_RAX = 3) by lia. clear BC. rewrite H in Cycles.
+        replace (n - 2) with (1 + (n - 3)) by lia. lia.
+        change (2^64) with (2^32 * 2^32). rewrite <- N.square_lt_mono.
+        lia.
+Qed.
+
+End TimingProof.
+        
+
